src/ShouldBuild.v
@@ -8,6 +8,8 @@ From Perennial.goose_lang Require
      refinement refinement_adequacy
      crash_lock
      logical_reln.
+From Perennial.goose_lang.lib Require
+     typed_slice.typed_slice.
 From Perennial.program_proof Require
      marshal_proof
      append_log_proof
