src/goose_lang/lib/typed_slice/typed_slice.v
@@ -1,0 +1,96 @@
+From Perennial.goose_lang Require Import notation proofmode typing.
+From Perennial.goose_lang.lib Require Import typed_mem.
+From Perennial.goose_lang.lib Require Import slice.impl.
+From Perennial.goose_lang.lib Require Import slice.slice.
+From Perennial.goose_lang.lib Require Import into_val.
+
+Module list.
+  Definition untype `{IntoVal V}:
+    list V -> list val := fun l => to_val <$> l.
+End list.
+
+Section heap.
+Context `{ffi_sem: ext_semantics} `{!ffi_interp ffi} `{!heapG Σ}.
+Context {ext_ty: ext_types ext}.
+
+Context `{!IntoVal V}.
+
+Implicit Types (s:Slice.t) (vs: list V) (v:V).
+Implicit Types (t:ty).
+
+Definition is_slice s t q vs := slice.is_slice s t q (list.untype vs).
+Definition is_slice_small s t q vs := slice.is_slice_small s t q (list.untype vs).
+
+Lemma is_slice_small_acc s t q vs :
+  is_slice s t q vs -∗ is_slice_small s t q vs ∗ (∀ vs', is_slice_small s t q vs' -∗ is_slice s t q vs').
+Proof.
+  iIntros "Hs".
+  iDestruct (slice.is_slice_small_acc with "Hs") as "[$ Hs]".
+  iIntros (vs') "Hsmall".
+  iApply ("Hs" with "[$]").
+Qed.
+
+Lemma is_slice_small_read s t q vs :
+  is_slice s t q vs -∗ is_slice_small s t q vs ∗ (is_slice_small s t q vs -∗ is_slice s t q vs).
+Proof.
+  iIntros "Hs".
+  iDestruct (slice.is_slice_small_read with "Hs") as "[$ Hs]".
+  iIntros "Hsmall".
+  iApply ("Hs" with "[$]").
+Qed.
+
+Lemma untype_replicate n x :
+  list.untype (replicate n x) = replicate n (to_val x).
+Proof.
+  rewrite /list.untype fmap_replicate //.
+Qed.
+
+Lemma wp_NewSlice stk E t `{!IntoValForType IntoVal0 t} (sz: u64) :
+  {{{ True }}}
+    NewSlice t #sz @ stk; E
+  {{{ s, RET slice_val s; is_slice s t 1 (replicate (int.nat sz) IntoVal_def) }}}.
+Proof.
+  iIntros (Φ) "_ HΦ".
+  wp_apply slice.wp_new_slice.
+  { apply to_val_has_zero. }
+  iIntros (s) "Hs".
+  iApply "HΦ".
+  rewrite /is_slice.
+  rewrite untype_replicate.
+  rewrite def_is_zero.
+  iApply "Hs".
+Qed.
+
+Lemma wp_SliceGet stk E s t q vs (i: u64) v0 :
+  {{{ is_slice_small s t q vs ∗ ⌜ vs !! int.nat i = Some v0 ⌝ }}}
+    SliceGet t (slice_val s) #i @ stk; E
+  {{{ RET to_val v0; is_slice_small s t q vs }}}.
+Proof.
+  iIntros (Φ) "[Hs %] HΦ".
+  iApply (slice.wp_SliceGet with "[$Hs]").
+  { iPureIntro.
+    rewrite /list.untype list_lookup_fmap.
+    rewrite H; eauto. }
+  iIntros "!> [Hs _]".
+  iApply ("HΦ" with "[$]").
+Qed.
+
+Lemma wp_SliceAppend stk E s t `{!IntoValForType IntoVal0 t} vs (x: V) :
+  {{{ is_slice s t 1 vs ∗ ⌜int.val s.(Slice.sz) + 1 < 2^64⌝ }}}
+    SliceAppend t (slice_val s) (to_val x) @ stk; E
+  {{{ s', RET slice_val s'; is_slice s' t 1 (vs ++ [x]) }}}.
+Proof.
+  iIntros (Φ) "[Hs %] HΦ".
+  wp_apply (slice.wp_SliceAppend with "[$Hs]").
+  { apply to_val_has_zero. }
+  { iSplit; first by auto.
+    iPureIntro.
+    apply to_val_ty. }
+  iIntros (s') "Hs".
+  rewrite /list.untype.
+  change [to_val x] with (to_val <$> [x]).
+  rewrite -fmap_app.
+  iApply ("HΦ" with "Hs").
+Qed.
+
+End heap.
